cedar-lean/Cedar/Thm/Validation/Typechecker/GetAttr.lean
@@ -37,31 +37,46 @@ theorem getAttrInRecord_has_empty_capabilities {x₁ : Expr} {a : Attr} {c₁ c�
   split at h₁ <;> simp at h₁
   simp [h₁]
 
-theorem type_of_getAttr_inversion {x₁ : Expr} {a : Attr} {c₁ c₂ : Capabilities} {env : Environment} {ty : CedarType}
-  (h₁ : typeOf (Expr.getAttr x₁ a) c₁ env = Except.ok (ty, c₂)) :
+theorem type_of_getAttr_inversion {x₁ : Expr} {a : Attr} {c₁ c₂ : Capabilities} {env : Environment} {ty : CedarType} {l : Level}
+  (h₁ : typeOf (Expr.getAttr x₁ a) c₁ env (l == .infinite) = Except.ok (ty, c₂)) :
   c₂ = ∅ ∧
   ∃ c₁',
-    (∃ ety, typeOf x₁ c₁ env = Except.ok (.entity ety, c₁')) ∨
-    (∃ rty, typeOf x₁ c₁ env = Except.ok (.record rty, c₁'))
+    (∃ ety l', typeOf x₁ c₁ env (l == .infinite) = Except.ok (.entity ety l', c₁')) ∨
+    (∃ rty, typeOf x₁ c₁ env (l == .infinite) = Except.ok (.record rty, c₁'))
 := by
   simp [typeOf] at h₁
-  cases h₂ : typeOf x₁ c₁ env <;> simp [h₂] at h₁
+  cases h₂ : typeOf x₁ c₁ env (l == .infinite) <;> simp [h₂] at h₁
   case ok res =>
     have ⟨ty₁, c₁'⟩ := res
     simp [typeOfGetAttr] at h₁
     split at h₁ <;> try contradiction
-    · simp only [List.empty_eq, Except.ok.injEq, Prod.mk.injEq, false_and, exists_const,
+    case _ =>
+      simp only [List.empty_eq, Except.ok.injEq, Prod.mk.injEq, false_and, exists_const,
         CedarType.record.injEq, exists_and_right, exists_eq', true_and, false_or, and_true]
       apply getAttrInRecord_has_empty_capabilities h₁
-    · simp only [List.empty_eq, Except.ok.injEq, Prod.mk.injEq, CedarType.entity.injEq,
-        exists_and_right, exists_eq', true_and, false_and, exists_const, or_false, and_true]
-      split at h₁ <;> try simp [err] at h₁
-      apply getAttrInRecord_has_empty_capabilities h₁
+    case _ =>
+      simp [*]
+      -- split on level being correct
+      split at h₁ <;> try contradiction
+      -- split at entity having this attribute
+      split at h₁ <;> try contradiction
+      simp [bind, Except.bind] at h₁
+      split at h₁ <;> try contradiction
+      rename_i tuple heq₂
+      cases tuple
+      rename_i ty caps
+      have heq₃ : caps = c₂ := by
+        simp at h₁
+        apply h₁.right
+      subst heq₃
+      apply getAttrInRecord_has_empty_capabilities
+      apply heq₂
 
-theorem type_of_getAttr_is_sound_for_records {x₁ : Expr} {a : Attr} {c₁ c₁' : Capabilities} {env : Environment} {rty : RecordType} {request : Request} {entities : Entities} {v₁ : Value}
+
+theorem type_of_getAttr_is_sound_for_records {x₁ : Expr} {a : Attr} {c₁ c₁' : Capabilities} {env : Environment} {rty : RecordType} {request : Request} {entities : Entities} {v₁ : Value} {l : Level}
   (h₁ : CapabilitiesInvariant c₁ request entities)
-  (h₂ : typeOf (Expr.getAttr x₁ a) c₁ env = Except.ok (ty, ∅))
-  (h₃ : typeOf x₁ c₁ env = Except.ok (CedarType.record rty, c₁'))
+  (h₂ : typeOf (Expr.getAttr x₁ a) c₁ env (l == .infinite) = Except.ok (ty, ∅))
+  (h₃ : typeOf x₁ c₁ env (l == .infinite) = Except.ok (CedarType.record rty, c₁'))
   (h₄ : evaluate x₁ request entities = Except.ok v₁)
   (h₅ : InstanceOfType v₁ (CedarType.record rty)) :
   ∃ v,
@@ -100,13 +115,97 @@ theorem type_of_getAttr_is_sound_for_records {x₁ : Expr} {a : Attr} {c₁ c₁
       subst h₂
       apply instance_of_attribute_type h₅ h₉ (by simp [Qualified.getType]) h₈
 
-theorem type_of_getAttr_is_sound_for_entities {x₁ : Expr} {a : Attr} {c₁ c₁' : Capabilities} {env : Environment} {ety : EntityType} {request : Request} {entities : Entities} {v₁ : Value}
+
+theorem setLevel_preserves_type {v : Value} {ty : CedarType} {l : Level}
+  (h : InstanceOfType v ty) :
+  InstanceOfType v (setLevel l.sub1 ty) := by
+  cases ty <;> cases v <;> cases h
+  case _ =>
+    simp [setLevel]
+    apply InstanceOfType.instance_of_bool
+    assumption
+  case _ =>
+    apply InstanceOfType.instance_of_int
+  case _ =>
+    apply InstanceOfType.instance_of_string
+  case _ =>
+    simp [setLevel]
+    apply InstanceOfType.instance_of_entity
+    assumption
+  case _ =>
+    simp [setLevel]
+    rename_i ty s h₁
+    apply InstanceOfType.instance_of_set
+    intros v h₂
+    apply setLevel_preserves_type
+    apply h₁
+    apply h₂
+  case _ =>
+    rename_i rty m h₁ h₂ h₃
+    simp [setLevel]
+      -- -- if an attribute is present in the record, then it is present in the type
+      -- (h₁ : ∀ (k : Attr), r.contains k → rty.contains k)
+      -- -- if an attribute is present, then it has the expected type
+      -- (h₂ : ∀ (k : Attr) (v : Value) (qty : QualifiedType),
+      --   r.find? k = some v → rty.find? k = some qty → InstanceOfType v qty.getType)
+      -- -- required attributes are present
+      -- (h₃ : ∀ (k : Attr) (qty : QualifiedType), rty.find? k = some qty → qty.isRequired → r.contains k) :
+      -- InstanceOfType (.record r) (.record rty)
+    apply InstanceOfType.instance_of_record
+    case _ =>
+      -- -- if an attribute is present in the record, then it is present in the type
+      -- (h₁ : ∀ (k : Attr), r.contains k → rty.contains k)
+      intros attr h₄
+      apply Map.mapOnValuesAttach_preservesKeys_adapter
+      apply h₁
+      apply h₄
+      exists (λ qual =>
+        match _h : qual with
+        | .required ty => .required (setLevel l.sub1 ty)
+        | .optional ty => .optional (setLevel l.sub1 ty)
+      )
+    case _ =>
+      -- -- if an attribute is present, then it has the expected type
+      -- (h₂ : ∀ (k : Attr) (v : Value) (qty : QualifiedType),
+      --   r.find? k = some v → rty.find? k = some qty → InstanceOfType v qty.getType)
+      intros k v qty h₄ h₅
+      sorry
+    case _ =>
+      sorry
+
+  case _ =>
+    simp [setLevel]
+    apply InstanceOfType.instance_of_ext
+    assumption
+termination_by sizeOf ty
+decreasing_by
+  all_goals simp_wf
+  all_goals try omega
+  case _ =>
+    rename_i c _ _ _ _ _ _ _ _ _ _ _ _ _
+    rw [c]
+    simp [sizeOf, CedarType._sizeOf_1]
+    omega
+  -- case _ =>
+  --   rename_i c _ _ _ _ _ _ _ _ _  _ _ _ _ _ _ _ _ _ _ _
+  --   rw [c]
+  --   simp [sizeOf, CedarType._sizeOf_1, Map._sizeOf_1, List._sizeOf_1]
+
+  --   omega
+
+
+    -- sorry
+
+
+
+
+theorem type_of_getAttr_is_sound_for_entities {x₁ : Expr} {a : Attr} {c₁ c₁' : Capabilities} {env : Environment} {ety : EntityType} {request : Request} {entities : Entities} {v₁ : Value} {l l₁ : Level}
   (h₁ : CapabilitiesInvariant c₁ request entities)
   (h₂ : RequestAndEntitiesMatchEnvironment env request entities)
-  (h₃ : typeOf (Expr.getAttr x₁ a) c₁ env = Except.ok (ty, ∅))
-  (h₄ : typeOf x₁ c₁ env = Except.ok (CedarType.entity ety, c₁'))
+  (h₃ : typeOf (Expr.getAttr x₁ a) c₁ env (l == .infinite) = Except.ok (ty, ∅))
+  (h₄ : typeOf x₁ c₁ env (l == .infinite) = Except.ok (CedarType.entity ety l₁, c₁'))
   (h₅ : evaluate x₁ request entities = Except.ok v₁)
-  (h₆ : InstanceOfType v₁ (CedarType.entity ety)) :
+  (h₆ : InstanceOfType v₁ (CedarType.entity ety l₁)) :
   ∃ v,
   (getAttr v₁ a entities = Except.error Error.entityDoesNotExist ∨
    getAttr v₁ a entities = Except.error Error.extensionError ∨
@@ -126,39 +225,66 @@ theorem type_of_getAttr_is_sound_for_entities {x₁ : Expr} {a : Attr} {c₁ c�
     simp only [Except.bind_ok]
     cases h₉ : Map.find? d.attrs a
     case none =>
-      simp only [Except.error.injEq, or_self, false_and, exists_const]
-      simp only [typeOf, h₄, typeOfGetAttr, getAttrInRecord, List.empty_eq, Except.bind_ok] at h₃
-      split at h₃ <;> simp [ok, err] at h₃
-      split at h₃ <;> try simp at h₃
-      case h_1.h_1 _ _ h₁₀ _ _ h₁₁ =>
-        subst h₃
+      simp
+      simp [typeOf, typeOfGetAttr, *] at h₃
+      split at h₃ <;> try contradiction
+      split at h₃  <;> try simp [err] at h₃
+      simp [getAttrInRecord] at *
+      split at h₃
+      case _ =>
+        simp [Except.bind, setLevel, ok] at h₃
+        rename_i h₁₀ _ _ h₁₁
         have h₁₂ := well_typed_entity_attributes h₂ h₈ h₁₀
-        have ⟨aᵥ, h₁₃⟩ := required_attribute_is_present h₁₂ h₁₁
+        have ⟨v, h₁₃⟩ := required_attribute_is_present h₁₂ h₁₁
         simp [h₉] at h₁₃
-      case h_1.h_2 =>
-        split at h₃ <;> simp at h₃
-        subst h₃ ; rename_i h₁₃
-        have ⟨_, h₁₄⟩ := capability_implies_entity_attribute h₁ h₅ h₈ h₁₃
-        simp [h₉] at h₁₄
-    case some vₐ =>
+      case _ =>
+        split at h₃
+        case _ =>
+          simp [ok, Except.bind] at h₃
+          rename_i hin
+          have ⟨_, h₁₀⟩  := capability_implies_entity_attribute h₁ h₅ h₈ hin
+          simp [h₉] at h₁₀
+        case _ =>
+          simp [err, Except.bind] at h₃
+      case _ =>
+        simp [err, Except.bind] at h₃
+    case _ =>
+      rename_i val
       simp only [Except.ok.injEq, false_or, exists_eq_left']
       simp [typeOf, h₄, typeOfGetAttr, getAttrInRecord] at h₃
       split at h₃ <;> simp [ok, err] at h₃
-      split at h₃ <;> try simp at h₃
-      case h_1.h_1 _ _ h₁₀ _ _ h₁₁ =>
-        subst h₃
-        apply instance_of_attribute_type _ h₁₁ (by simp [Qualified.getType]) h₉
-        apply well_typed_entity_attributes h₂ h₈ h₁₀
-      case h_1.h_2 _ _ h₁₀ _ _ h₁₁ =>
-        split at h₃ <;> simp at h₃
-        subst h₃
-        apply instance_of_attribute_type _ h₁₁ (by simp [Qualified.getType]) h₉
-        apply well_typed_entity_attributes h₂ h₈ h₁₀
+      split at h₃ <;> try simp [ok, err] at h₃
+      split at h₃ <;> try simp [Except.bind] at h₃
+      case _ =>
+        rename_i heq _ _ _
+        have h_entity := well_typed_entity_attributes h₂ h₈ heq
+        rename_i attrTy heq₁
+        have h_step : InstanceOfType val attrTy := by
+          apply instance_of_attribute_type
+          apply h_entity
+          assumption
+          simp [Qualified.getType]
+          assumption
+        rw [← h₃]
+        apply setLevel_preserves_type h_step
+      case _ =>
+        split at h₃ <;> simp [Except.bind] at h₃
+        rename_i heq₁ qual attrTy heq₂  hin
+        have h_entity := well_typed_entity_attributes h₂ h₈ heq₁
+        have h_step : InstanceOfType val attrTy := by
+          apply instance_of_attribute_type
+          apply h_entity
+          assumption
+          simp [Qualified.getType]
+          assumption
+        rw [← h₃]
+        apply setLevel_preserves_type h_step
 
-theorem type_of_getAttr_is_sound {x₁ : Expr} {a : Attr} {c₁ c₂ : Capabilities} {env : Environment} {ty : CedarType} {request : Request} {entities : Entities}
+
+theorem type_of_getAttr_is_sound {x₁ : Expr} {a : Attr} {c₁ c₂ : Capabilities} {env : Environment} {ty : CedarType} {request : Request} {entities : Entities} {l : Level}
   (h₁ : CapabilitiesInvariant c₁ request entities)
   (h₂ : RequestAndEntitiesMatchEnvironment env request entities)
-  (h₃ : typeOf (Expr.getAttr x₁ a) c₁ env = Except.ok (ty, c₂))
+  (h₃ : typeOf (Expr.getAttr x₁ a) c₁ env (l == .infinite) = Except.ok (ty, c₂))
   (ih : TypeOfIsSound x₁) :
   GuardedCapabilitiesInvariant (Expr.getAttr x₁ a) c₂ request entities ∧
   ∃ v, EvaluatesTo (Expr.getAttr x₁ a) request entities v ∧ InstanceOfType v ty
@@ -166,11 +292,11 @@ theorem type_of_getAttr_is_sound {x₁ : Expr} {a : Attr} {c₁ c₂ : Capabilit
   have ⟨h₅, c₁', h₄⟩ := type_of_getAttr_inversion h₃
   subst h₅
   apply And.intro empty_guarded_capabilities_invariant
-  rcases h₄ with ⟨ety, h₄⟩ | ⟨rty, h₄⟩ <;>
+  rcases h₄ with ⟨ety, l', h₄⟩ | ⟨rty, h₄⟩  <;>
   have ⟨_, v₁, h₆, h₇⟩ := ih h₁ h₂ h₄ <;>
-  simp [EvaluatesTo] at h₆ <;>
-  simp [EvaluatesTo, evaluate] <;>
-  rcases h₆ with h₆ | h₆ | h₆ | h₆ <;> simp [h₆]
+  try simp [EvaluatesTo] at h₆ <;>
+  try simp [EvaluatesTo, evaluate] <;>
+  try rcases h₆ with h₆ | h₆ | h₆ | h₆ <;> simp [h₆]
   <;> try exact type_is_inhabited ty
   · exact type_of_getAttr_is_sound_for_entities h₁ h₂ h₃ h₄ h₆ h₇
   · exact type_of_getAttr_is_sound_for_records h₁ h₃ h₄ h₆ h₇
